PDDL-sema/Util.thy
@@ -1,0 +1,55 @@
+theory Util
+  imports Main
+begin
+context comp_fun_commute_on
+begin
+
+find_theorems name: "local*fold"
+thm fold_fun_left_comm
+
+lemma list_fold_left_comm:
+  assumes "set (x # xs) \<subseteq> S"
+  shows "f x (fold f xs B) = fold f xs (f x B)"
+  using assms
+proof (induction xs arbitrary: B)
+  case Nil
+  then show ?case by simp
+next
+  case (Cons a xs)
+  have "f x (fold f (a # xs) B) = f x (fold f xs (f a B))"
+    by simp            
+  also have "... = fold f xs (f x (f a B))" using Cons by simp
+  also have "... = fold f xs (f a (f x B))" 
+    using Cons 
+    apply (subst comp_apply[of "f x" "f a", symmetric])
+    apply (subst comp_fun_commute_on[where x = a and y = x])
+    by auto
+  finally show ?case by simp
+qed
+
+lemma fold_rev:
+  assumes "set xs \<subseteq> S"
+  shows "fold f xs = fold f (rev xs)"
+  using assms
+proof (induction xs)
+  case Nil
+  then show ?case by simp
+next
+  case (Cons x xs)
+  have "fold f (x # xs) = f x o (fold f xs)" 
+    using list_fold_left_comm Cons by auto
+  also have "... = f x o (fold f (rev xs))" using Cons by auto
+  also have "... = f x o (fold id (map f (rev xs)))" 
+    apply (subst fold_map[of id, simplified id_comp, symmetric])
+    ..
+  also have "... = (id (f x)) o (fold id (map f (rev xs)))" by simp
+  also have "... = fold id (map f ((rev xs)@[x]))" by simp
+  finally show ?case 
+    apply (subst rev.simps(2))
+    apply (subst (asm) fold_map[of id, simplified id_comp])
+    by simp
+qed
+end
+
+
+end
